add sismo

src/CircomLib/Comparators.v
@@ -216,6 +216,65 @@ Proof.
     lia.
 Qed.
 
+Lemma soundness': forall (w : t),
+  (* pre-conditions: both inputs are at most (k-1) bits *)
+  (n <= C.k - 1)%Z ->
+  (^ w.(_in)[0] <= 2^n)%Z ->
+  (^ w.(_in)[1] <= 2^n)%Z  ->
+  (* post-condition *)
+  binary w.(out) /\
+  let '(x, y) := (w.(_in)[0], w.(_in)[1]) in
+  if (w.(out) = 1)? then
+    x <q y
+  else
+    x >=q y.
+Proof.
+  unwrap_C. intros w H_nk Hx Hy.
+  remember (w.(_in)[0]) as x. remember (w.(_in)[1]) as y.
+  destruct w as [_in out [n2b H]]. simpl in *.
+  rewrite <- Heqx, <- Heqy in *.
+  pose proof (Num2Bits.soundness n2b) as H_n2b.
+  pose proof H_n2b as H_n2b'.
+  unfold repr_le2, repr_le in H_n2b.
+  destruct H as [H_n Hout ].
+  apply conj_use.
+  intuition.
+  - eapply one_minus_binary; eauto.
+    rewrite nth_Default_nth_default, <- nth_default_to_list, nth_default_eq. 
+    apply Forall_nth. apply Forall_in_range. auto.
+    lia.
+  - assert (H_pow_nk: (2 * 2^n <= 2^k)%Z). {
+      replace (2 * 2^n)%Z with (2 ^ (n + 1))%Z by (rewrite Zpower_exp; lia).
+      apply Zpow_facts.Zpower_le_monotone; lia.
+    }
+    assert (H_x_nonneg: (0 <= F.to_Z x)%Z). apply F.to_Z_range. lia.
+    assert (H_y_nonneg: (0 <= F.to_Z y)%Z). apply F.to_Z_range. lia.
+    destruct (dec (out = 1)).
+    + assert (Hn: Num2Bits.out n2b [n] = 0) by fqsatz.
+      rewrite nth_Default_nth_default, <- nth_default_to_list, nth_default_eq in Hn.
+      remember (to_list (S n) (Num2Bits.out n2b)) as n2bout.
+        unfold repr_le2 in *.
+        eapply repr_le_last0' in Hn. 2: { rewrite H_n in H_n2b'. apply H_n2b'. }
+        fold repr_le2 in Hn.
+        apply repr_le_ub in Hn; try lia.
+      assert (F.to_Z x + 2^n - F.to_Z y <= 2^n - 1 )%Z. {
+        autorewrite with F_to_Z in Hn; try lia;
+        repeat autorewrite with F_to_Z; simpl; try lia.
+        simpl in Hn. lia.
+      }
+      lia.
+    + destruct H0; try fqsatz. assert (Hn: Num2Bits.out n2b [n] = 1) by fqsatz.
+    rewrite H_n in *.
+    rewrite nth_Default_nth_default, <- nth_default_to_list, nth_default_eq in Hn.
+    eapply repr_le_lb with (i:=n) in Hn; eauto; try lia.
+    assert (F.to_Z x + 2^n - F.to_Z y >= 2^n)%Z. {
+      autorewrite with F_to_Z in Hn; try lia;
+      repeat autorewrite with F_to_Z; simpl; try lia.
+      simpl in Hn. lia.
+    }
+    lia.
+Qed.
+
 Lemma is_binary: forall (w:t), 
   (n <= C.k - 1)%Z ->
   w.(_in)[0] | (n) ->
@@ -255,5 +314,72 @@ Definition wgen: LessThan.t. skip. Defined.
 
 End LessThan.
 End LessThan.
+
+(***********************
+ *       LessThanEq
+ ***********************)
+Module LessEqThan.
+
+Section LessEqThan.
+Context {n: nat}.
+
+(* template LessEqThan(n) {
+    signal input in[2];
+    signal output out;
+
+    component lt = LessThan(n);
+
+    lt.in[0] <== in[0];
+    lt.in[1] <== in[1]+1;
+    lt.out ==> out;
+} *)
+
+Definition cons (in_: F^2) (out: F) :=
+  exists (lt: @LessThan.t n),
+    lt.(LessThan._in)[0] = in_[0] /\
+    lt.(LessThan._in)[1] = in_[1] + 1 /\
+    lt.(LessThan.out) = out.
+
+Record t: Type := {
+  _in: F^2;
+  out: F;
+  _cons: cons _in out;
+}.
+
+Lemma soundness : forall (w: t),
+  (n <= C.k - 1)%Z ->
+  w.(_in)[0] | (n) ->
+  w.(_in)[1] | (n) ->
+  binary w.(out) /\
+  let '(x, y) := (w.(_in)[0], w.(_in)[1]) in
+  if (w.(out) = 1)? then
+    x <=q y
+  else
+    x >q y.
+Proof.
+  intros. 
+  destruct w as [w_in w_out [lt [H_lt_in0 [H_lt_in1 H_lt_out]]]].
+  pose proof (@F.to_Z_range q (w_in [0])) as hhh1. 
+  pose proof (@F.to_Z_range q (w_in [1])) as hhh2. 
+  simpl in *. pose proof two_lt_q. pose proof q_lb as q_lb.
+  pose proof (LessThan.soundness' lt) as H_lt.
+  unfold LessThan.cons in H_lt.
+  subst. rewrite H_lt_in0, H_lt_in1 in *.
+  assert (Hndm: (2 ^ n <= 2^k)%Z). apply Zpow_facts.Zpower_le_monotone; lia.
+  destruct H_lt;auto;try lia. 
+  { unfold F.to_Z. simpl. do 2 rewrite Zmod_small;try lia. }
+  split; auto.
+  destruct (dec (LessThan.out lt = 1)).
+  - apply Ztac.Zlt_le_add_1 in H4. simpl in *.
+    rewrite Zmod_small in H4 at 1. 
+    2:{ rewrite Zmod_small;try lia. } 
+    rewrite Zmod_small in H4 at 1;lia.
+  - simpl in *. rewrite Zmod_small in H4 at 1. 
+    2:{ rewrite Zmod_small;try lia. }
+    rewrite Zmod_small in H4 at 1;lia. 
+Qed.
+
+End LessEqThan.
+End LessEqThan.
 
 End Comparators.
